Examples/OneTimePad.lean
@@ -12,37 +12,21 @@ import Mathlib.Data.Vector.Zip
 This file defines and proves the perfect secrecy of the one-time pad encryption algorithm.
 -/
 
-open Mathlib OracleSpec OracleComp OracleAlg ENNReal BigOperators
+open Mathlib OracleSpec OracleComp OracleImpl ENNReal BigOperators
 
 /-- The one-time pad symmetric encryption algorithm, using `BitVec`s as keys and messages.
 Encryption and decryption both just apply `BitVec.xor` with the key.
 Requires no oracles so the `OracleSpec` is always `[]ₒ`. -/
-def oneTimePad' (n : ℕ) : SymmEncAlg' []ₒ Unit
-    (BitVec n) (BitVec n) (BitVec n) where
+@[simps!] def oneTimePad (n : ℕ) : SymmEncAlg unifSpec Unit
+    (M := BitVec n) (K := BitVec n) (C := BitVec n) where
   keygen := $ᵗ BitVec n
   encrypt k m := return k ^^^ m
   decrypt k σ := return k ^^^ σ
-  __ := emptyImpl
-
-/-- The one-time pad symmetric encryption algorithm, using `BitVec`s as keys and messages.
-Encryption and decryption both just apply `BitVec.xor` with the key.
-Requires no oracles so the `OracleSpec` is always `[]ₒ`. -/
-def oneTimePad : SymmEncAlg (λ _ ↦ []ₒ) BitVec BitVec BitVec where
-  keygen n := $ᵗ BitVec n
-  encrypt _ k m := return k ^^^ m
-  decrypt _ k σ := return k ^^^ σ
-  __ := baseOracleAlg
+  __ := defaultImpl
 
 namespace oneTimePad
 
-@[simp]
-lemma keygen_def (n : ℕ) : oneTimePad.keygen n = $ᵗ BitVec n := rfl
-
-@[simp]
-lemma encrypt_bind_decrypt {n : ℕ} (k m : BitVec n) :
-    do {let σ ← oneTimePad.encrypt _ k m; oneTimePad.decrypt _ k σ} = return m := by
-  simp [oneTimePad]
-
-theorem isSound : oneTimePad.isSound := λ sp m ↦ probOutput_eq_one (by simp)
+theorem isComplete (n : ℕ) : (oneTimePad n).isComplete :=
+  λ m ↦ probOutput_eq_one (by simp [SymmEncAlg.soundnessExp])
 
 end oneTimePad
