VCVio/CryptoFoundations/AsymmEncAlg.lean
@@ -5,7 +5,6 @@ Authors: Devon Tuma
 -/
 import VCVio.CryptoFoundations.SecExp
 import VCVio.OracleComp.Constructions.UniformSelect
-import VCVio.OracleComp.Coercions.Append
 
 /-!
 # Asymmetric Encryption Schemes.
@@ -17,87 +16,99 @@ public/secret keys `PK` and `SK`, and ciphertext space `C`.
 
 open OracleSpec OracleComp
 
-structure AsymmEncAlg {ι : Type} (spec : ℕ → OracleSpec ι)
-    (M PK SK C : ℕ → Type)
-    extends OracleAlg spec where
-  keygen (sp : ℕ) : OracleComp (unifSpec ++ₒ spec sp) (PK sp × SK sp)
-  encrypt (sp : ℕ) : M sp → PK sp → OracleComp (unifSpec ++ₒ spec sp) (C sp)
-  decrypt (sp : ℕ) : C sp → SK sp → OracleComp (unifSpec ++ₒ spec sp) (M sp)
+structure AsymmEncAlg {ι : Type} (spec : OracleSpec ι)
+    (σ M PK SK C : Type) extends OracleImpl spec σ where
+  keygen : OracleComp spec (PK × SK)
+  encrypt (m : M) (pk : PK) : OracleComp spec C
+  decrypt (c : C) (sk : SK) : OracleComp spec M
 
 namespace AsymmEncAlg
 
-variable {ι : Type} {spec : ℕ → OracleSpec ι} {M PK SK C : ℕ → Type}
+variable {ι : Type} {spec : OracleSpec ι} {σ M PK SK C : Type}
 
 section sound
 
-variable [Π sp, DecidableEq (M sp)]
+-- variable [Π sp, DecidableEq (M sp)]
 
-/-- Experiment for checking that an asymmetric encryption algorithm is sound,
-i.e. that decryption properly reverses encryption -/
-def soundnessExp (encAlg : AsymmEncAlg spec M PK SK C)
-    (mDist : (sp : ℕ) → OracleComp (spec sp) (M sp)) :
-    SecExp spec where
-  main := λ sp ↦ do
-    let m ← mDist sp
-    let (pk, sk) ← encAlg.keygen sp
-    let σ ← encAlg.encrypt sp m pk
-    let m' ← encAlg.decrypt sp σ sk
-    return m = m'
+
+-- /-- Experiment for checking that an asymmetric encryption algorithm is sound,
+-- i.e. that decryption properly reverses encryption -/
+-- def soundnessExp (encAlg : AsymmEncAlg spec M PK SK C)
+--     (mDist : (sp : ℕ) → OracleComp (spec sp) (M sp)) :
+--     SecExp spec where
+--   main := λ sp ↦ do
+--     let m ← mDist sp
+--     let (pk, sk) ← encAlg.keygen sp
+--     let σ ← encAlg.encrypt sp m pk
+--     let m' ← encAlg.decrypt sp σ sk
+--     return m = m'
+--   __ := encAlg
+
+def soundnessExp [DecidableEq M] (encAlg : AsymmEncAlg spec σ M PK SK C)
+    (m : M) : SecExp spec σ where
+  main := do
+    let (pk, sk) ← encAlg.keygen
+    let σ ← encAlg.encrypt m pk
+    let m' ← encAlg.decrypt σ sk
+    return m' = m
   __ := encAlg
 
-namespace soundnessExp
+def IsSound [DecidableEq M] (encAlg : AsymmEncAlg spec σ M PK SK C) : Prop :=
+  ∀ m : M, (soundnessExp encAlg m).advantage = 1
+
+-- namespace soundnessExp
 
 
-end soundnessExp
+-- end soundnessExp
 
-/-- An asymmetric encryption algorithm is sound if messages always decrypt to themselves. -/
-def isSound (encAlg : AsymmEncAlg spec M PK SK C) : Prop :=
-  ∀ mDist, negligible (1 - (soundnessExp encAlg mDist).advantage)
+-- /-- An asymmetric encryption algorithm is sound if messages always decrypt to themselves. -/
+-- def isSound (encAlg : AsymmEncAlg spec M PK SK C) : Prop :=
+--   ∀ mDist, negligible (1 - (soundnessExp encAlg mDist).advantage)
 
--- lemma sound_iff [DecidableEq M] (encAlg : AsymmEncAlg spec M PK SK C) : encAlg.isSound ↔
---     ∀ m : M, ∀ m' ∈ (encAlg.exec <| do
---       let (pk, sk) ← encAlg.keygen ()
---       let σ ← encAlg.encrypt m pk
---       encAlg.decrypt σ sk).support, m = m' := by
---   simp only [isSound, SecExp.advantage_eq_one_iff]
---   sorry
+-- -- lemma sound_iff [DecidableEq M] (encAlg : AsymmEncAlg spec M PK SK C) : encAlg.isSound ↔
+-- --     ∀ m : M, ∀ m' ∈ (encAlg.exec <| do
+-- --       let (pk, sk) ← encAlg.keygen ()
+-- --       let σ ← encAlg.encrypt m pk
+-- --       encAlg.decrypt σ sk).support, m = m' := by
+-- --   simp only [isSound, SecExp.advantage_eq_one_iff]
+-- --   sorry
 
 end sound
 
-section IND_CPA
+-- section IND_CPA
 
-variable [DecidableEq ι]
+-- variable [DecidableEq ι]
 
-/-- `IND_CPA_adv M PK C` is an adversary for IND-CPA security game on an
-asymmetric encryption algorithm with public keys in `PK`, messages in `M`, and ciphertexts in `C`.
-Adversary is given a public key and returns a pair of messages that it thinks
-it can distinguish the encryption of. It addionally has a `distinguish` function
-that given a pair of messages and an encryption, returns whether it is an encryption of
-the first message or the second message. -/
-structure IND_CPA_Adv (encAlg : AsymmEncAlg spec M PK SK C)
-    extends SecAdv spec (λ sp ↦ PK sp) (λ sp ↦ M sp × M sp) where
-  distinguish (sp : ℕ) : PK sp → M sp × M sp →
-    C sp → OracleComp (spec sp) Bool
+-- /-- `IND_CPA_adv M PK C` is an adversary for IND-CPA security game on an
+-- asymmetric encryption with public keys in `PK`, messages in `M`, and ciphertexts in `C`.
+-- Adversary is given a public key and returns a pair of messages that it thinks
+-- it can distinguish the encryption of. It addionally has a `distinguish` function
+-- that given a pair of messages and an encryption, returns whether it is an encryption of
+-- the first message or the second message. -/
+-- structure IND_CPA_Adv (encAlg : AsymmEncAlg spec M PK SK C)
+--     extends SecAdv spec (λ sp ↦ PK sp) (λ sp ↦ M sp × M sp) where
+--   distinguish (sp : ℕ) : PK sp → M sp × M sp →
+--     C sp → OracleComp (spec sp) Bool
 
-/-- Experiment for IND-CPA security of an asymmetric encryption algorithm.
-`inp_gen` generates a key and pre-selects a random boolean value.
-`main` runs the adversary on the public key, and encrypts the resulting message corresponding to
-the boolean chosen in `inp_gen`, finally asking the adversary to determine the boolean
-given the messages and resulting ciphertext. `is_valid` checks that this choice is correct.
-The simulation oracles are pulled in directly from the encryption algorithm. -/
-def IND_CPA_Exp {encAlg : AsymmEncAlg spec M PK SK C}
-    (adv : IND_CPA_Adv encAlg) :
-    SecExp spec where
-  main := λ sp ↦ do
-    let (pk, _) ← encAlg.keygen sp
-    let (m₁, m₂) ← adv.run sp pk
-    let b : Bool ← coin
-    let m := if b then m₁ else m₂
-    let c ← encAlg.encrypt sp m pk
-    let b' ← adv.distinguish sp pk (m₁, m₂) c
-    return b = b'
-  __ := encAlg
+-- /-- Experiment for IND-CPA security of an asymmetric encryption algorithm.
+-- `inp_gen` generates a key and pre-selects a random boolean value.
+-- `main` runs the adversary on the public key, and encrypts the resulting message corresponding to
+-- the boolean chosen in `inp_gen`, finally asking the adversary to determine the boolean
+-- given the messages and resulting ciphertext. `is_valid` checks that this choice is correct.
+-- The simulation oracles are pulled in directly from the encryption algorithm. -/
+-- def IND_CPA_Exp {encAlg : AsymmEncAlg spec M PK SK C}
+--     (adv : IND_CPA_Adv encAlg) :
+--     SecExp spec where
+--   main := λ sp ↦ do
+--     let (pk, _) ← encAlg.keygen sp
+--     let (m₁, m₂) ← adv.run sp pk
+--     let b : Bool ← coin
+--     let m := if b then m₁ else m₂
+--     let c ← encAlg.encrypt sp m pk
+--     let b' ← adv.distinguish sp pk (m₁, m₂) c
+--     return b = b'
+--   __ := encAlg
 
-end IND_CPA
+-- end IND_CPA
 
 end AsymmEncAlg
