VCVio/CryptoFoundations/Fork.lean
@@ -4,15 +4,16 @@ Released under Apache 2.0 license as described in the file LICENSE.
 Authors: Devon Tuma
 -/
 import VCVio.CryptoFoundations.SecExp
--- import VCVio.OracleComp.Constructions.GenerateSeed
--- import VCVio.OracleComp.OracleSpec.SubSpec
+import VCVio.OracleComp.Constructions.GenerateSeed
+import VCVio.OracleComp.SimSemantics.QueryTracking.LoggingOracle
+import VCVio.OracleComp.Coercions.Append
 
 /-!
 # Forking Lemma
 
 -/
 
-open OracleSpec OracleComp OracleAlg Option ENNReal
+open OracleSpec OracleComp Option ENNReal
 
 -- structure ForkAdv {ι : Type} (spec : OracleSpec ι) (α β : Type) (i : ι)
 --     extends SecAdv spec α β where
@@ -39,46 +40,52 @@ namespace OracleComp
 -- variable {ι : Type} [DecidableEq ι] {spec : OracleSpec ι} [∀ j, SelectableType (spec.range j)]
 --   [unifSpec ⊂ₒ spec] {α β : Type} {i : ι}
 
--- -- def fork (adv : ForkAdv spec α β i) :
--- --     SecAdv spec α (Option (β × β)) where
--- --   run := λ x ↦ do
--- --     -- pre-select where to fork execution
--- --     let s : Fin _ ← $[0..adv.queryBound i]
--- --     let qc := Function.update adv.queryBound i s
--- --     -- Generate shared seed for both runs
--- --     let sharedSeed : QuerySeed spec ← ↑(generateSeed qc adv.activeOracles)
--- --     -- Add the forked queries to the two seeds
--- --     let seed₁ ← sharedSeed.addValue i <$> ($ᵗ spec.range i)
--- --     let seed₂ ← sharedSeed.addValue i <$> ($ᵗ spec.range i)
--- --     -- Run the adversary on both seeds
--- --     let y₁ ← simulate' seededOracle seed₁ (adv.run x)
--- --     let y₂ ← simulate' seededOracle seed₂ (adv.run x)
--- --     -- Only return a value on success
--- --     if adv.chooseFork x y₁ = some s ∧
--- --         adv.chooseFork x y₂ = some s ∧
--- --         (seed₁ i).getI s ≠ (seed₂ i).getI s
--- --       then return some (y₁, y₂)
--- --       else return none
--- --   queryBound := 2 • adv.queryBound
--- --   activeOracles := adv.activeOracles
+variable {ι : Type} [DecidableEq ι] {spec : OracleSpec ι} {α β γ : Type}
 
--- theorem some_mem_support_fork_iff (adv : ForkAdv spec α β i) (x : α) (y₁ y₂ : β)
---     (h : some (y₁, y₂) ∈ ((fork adv).run x).support) :
---     ∃ s : Fin (adv.queryBound i + 1), ∃ seed₁ seed₂ : QuerySeed spec,
---       ∃ h₁ : ↑s < (seed₁ i).length, ∃ h₂ : ↑s < (seed₂ i).length,
---         (seed₁ i)[↑s]'h₁ ≠ (seed₂ i)[↑s]'h₂ ∧
---         y₁ ∈ (simulate' seededOracle seed₁ (adv.run x)).support ∧
---         y₂ ∈ (simulate' seededOracle seed₂ (adv.run x)).support ∧
---         adv.chooseFork x y₁ = some s ∧ adv.chooseFork x y₂ = some s :=
---   alignPort
+instance {ι : Type} (spec : OracleSpec ι) [unifSpec ⊂ₒ spec] (α : Type) :
+    Coe (ProbComp α) (OracleComp spec α) where
+  coe := λ oa ↦ SubSpec.liftComp oa
 
--- theorem le_fork_advantage
---     (adv : ForkAdv spec α β i) (x : α) :
---     let frk := [(· ≠ none) | (fork adv).run x]
---     let acc := [(· ≠ none) | adv.chooseFork x <$> adv.run x]
---     let q : ℝ≥0∞ := adv.queryBound i + 1
---     let h : ℝ≥0∞ := Fintype.card (spec.range i)
---     (acc / q) ^ 2 - acc / h ≤ frk :=
---   alignPort
+variable [∀ i, SelectableType (spec.range i)]
+
+def fork [unifSpec ⊂ₒ spec] (oa : OracleComp spec α) (qb : ι → ℕ)
+    (activeOracles : List ι) (i : ι)
+    (cf : α → Option (Fin (qb i + 1))) :
+    OracleComp spec (Option (α × α × Fin (qb i + 1))) := do
+  let s : Fin (qb i + 1) ← $[0..qb i]
+  let sharedSeed : QuerySeed spec ← generateSeed spec (Function.update qb i s) activeOracles
+  let seed₁ ← sharedSeed.addValue i <$> ($ᵗ spec.range i)
+  let seed₂ ← sharedSeed.addValue i <$> ($ᵗ spec.range i)
+  let y₁ ← simulate' seededOracle seed₁ oa
+  let y₂ ← simulate' seededOracle seed₂ oa
+  return if cf y₁ = some s ∧ cf y₂ = some s ∧ (seed₁ i).getI s ≠ (seed₂ i).getI s
+    then some (y₁, y₂, s) else none
+
+variable [unifSpec ⊂ₒ spec] (oa : OracleComp spec α) (qb : ι → ℕ)
+    (js : List ι) (i : ι)
+    (cf : α → Option (Fin (qb i + 1)))
+
+/-- Proof of non-negligible lower bound on the failure chance of forking a computation
+succeeding in producing a result. By the filtering in the final `ite` this bounds the
+chance of getting a result with the desired forking semantics. -/
+theorem le_probEvent_isSome_fork :
+    let frk := [λ z ↦ z.isSome | fork oa qb js i cf]
+    let acc := [λ z ↦ z.isSome | cf <$> oa]
+    let q : ℝ≥0∞ := qb i
+    let h : ℝ≥0∞ := Fintype.card (spec.range i)
+    (acc / q) ^ 2 - acc / h ≤ frk := by
+  sorry
+
+/-- Theorem expressing the most useful properties of successful forking.
+Weaker than the full characterization of the `support` of fork,
+but often more useful in practice -/
+theorem exists_log_of_mem_support_fork (x₁ x₂ : α) (s : Fin (qb i + 1))
+    (h : some (x₁, x₂, s) ∈ ((fork oa qb js i cf)).support) :
+    ∃ log₁ : QuerySeed spec, ∃ log₂ : QuerySeed spec,
+      (log₁ i).getI s ≠ (log₂ i).getI s ∧
+      cf x₁ = some s ∧ cf x₂ = some s ∧
+      x₁ ∈ (simulate' loggingOracle ∅ oa).support ∧
+      x₂ ∈ (simulate' loggingOracle ∅ oa).support :=
+  sorry
 
 end OracleComp
