VCVio/CryptoFoundations/SymmEncAlg.lean
@@ -14,82 +14,39 @@ for symmetric encryption using oracles in `spec`, with message space `M`,
 secret keys of type `K`, and ciphertext space `C`.
 -/
 
-open OracleSpec OracleComp OracleAlg BigOperators
+open OracleSpec OracleComp
 
-/-- An implementation of the oracles in `spec` gives a way to run all the oracles in `spec`.
-Allows a computation using `spec` to be simulated in terms of `unifSpec` to produce
-a `ProbComp` that can be run with `OracleComp.runIO`.
-
-The types of primitives can extend this to ensure that any oracles used in a protocol
-must have some canonical implementation. -/
-structure OracleImpl {ι : Type} (spec : OracleSpec ι) (σ : Type) where
-  baseSimOracle : spec →[σ]ₛₒ unifSpec
-  init_state : σ
-
-def OracleImpl.exec {ι : Type} {spec : OracleSpec ι} {α σ : Type}
-    (impl : OracleImpl spec σ) (oa : OracleComp (unifSpec ++ₒ spec) α) : ProbComp (α × σ) :=
-  let so := (idOracle ++ₛₒ impl.baseSimOracle).maskState <| Equiv.punitProd σ
-  simulate so impl.init_state oa
-
-def OracleImpl.exec' {ι : Type} {spec : OracleSpec ι} {α σ : Type}
-    (impl : OracleImpl spec σ) (oa : OracleComp (unifSpec ++ₒ spec) α) : ProbComp α :=
-  let so := (idOracle ++ₛₒ impl.baseSimOracle).maskState <| Equiv.punitProd σ
-  simulate' so impl.init_state oa
-
-def emptyImpl : OracleImpl []ₒ Unit where
-  baseSimOracle := unifOracle
-  init_state := ()
-
-structure SymmEncAlg' {ι : Type} (spec : OracleSpec ι) (σ M K C : Type)
+/-- Symmetric encryption algorithm with access to oracles in `spec` (simulated with state `σ`),
+where `M` is the space of messages, `K` is the key space, and `C` is the ciphertext space. -/
+structure SymmEncAlg {ι : Type} (spec : OracleSpec ι) (σ M K C : Type)
     extends OracleImpl spec σ where
-  keygen : OracleComp (unifSpec ++ₒ spec) K
-  encrypt (k : K) (m : M) : OracleComp (unifSpec ++ₒ spec) C
-  decrypt (k : K) (c : C) : OracleComp (unifSpec ++ₒ spec) M
-
-structure SymmEncAlg {ι : Type} (spec : ℕ → OracleSpec ι) (M K C : ℕ → Type)
-    extends OracleAlg spec where
-  (keygen (sp : ℕ) : OracleComp (unifSpec ++ₒ spec sp) (K sp))
-  (encrypt (sp : ℕ) : K sp → M sp → OracleComp (unifSpec ++ₒ spec sp) (C sp))
-  (decrypt (sp : ℕ) : K sp → C sp → OracleComp (unifSpec ++ₒ spec sp) (M sp))
+  keygen : OracleComp spec K
+  encrypt (k : K) (m : M) : OracleComp spec C
+  decrypt (k : K) (c : C) : OracleComp spec M
 
 namespace SymmEncAlg
 
-variable {ι : Type} {spec : ℕ → OracleSpec ι} {M K C : ℕ → Type}
+variable {ι : Type} {spec : OracleSpec ι} {σ M K C : Type}
 
-section isSound
+section sound
 
-variable [Π sp, DecidableEq (M sp)]
+variable [DecidableEq M]
 
-/-- A symmetric encryption algorithm is sound is messages decrypt to themselves given a random key.
-Note that we assume the algorithm never fails, although in general this could be modified
-to allow for a (negligible) chance of encryption failure. -/
-def isSound (encAlg : SymmEncAlg spec M K C) : Prop :=
-  ∀ sp : ℕ, ∀ m : M sp, [= m | do
-    let k ← encAlg.keygen sp
-    let σ ← encAlg.encrypt sp k m
-    encAlg.decrypt sp k σ] = 1
-
-def isSound' {ι : Type} {spec : OracleSpec ι} {σ M K C : Type}
-    (encAlg : SymmEncAlg' spec σ M K C) : Prop :=
-  ∀ m : M, [= m | Prod.fst <$> (encAlg.exec do
-    let k : K ← encAlg.keygen
+/-- Experiment to check that an encryption and decryption are inverses of each other. -/
+def soundnessExp (encAlg : SymmEncAlg spec σ M K C)
+    (m : M) : SecExp spec σ where
+  main := do
+    let k ← encAlg.keygen
     let σ ← encAlg.encrypt k m
-    encAlg.decrypt k σ)] = 1
+    let m' ← encAlg.decrypt k σ
+    return m' = m
+  __ := encAlg
 
-variable (encAlg : SymmEncAlg spec M K C)
+/-- A symmetric encryption algorithm is complete if correctly generated ciphertexts
+always decrypt to the original plaintext. -/
+def isComplete (encAlg : SymmEncAlg spec σ M K C) : Prop :=
+  ∀ m : M, (soundnessExp encAlg m).advantage = 1
 
--- lemma isSound_iff {ι : Type} {spec : OracleSpec ι} {M K C : Type}
---     (encAlg : SymmEncAlg' spec M K C) : encAlg.isSound ↔
---     ∀ m : M, ()
-
--- lemma isSound_iff_forall_mem_support :
-
-end isSound
-
--- section perfectSecrecy
-
-
-
--- end perfectSecrecy
+end sound
 
 end SymmEncAlg
