Test.lean
@@ -2,5 +2,7 @@
 import LibSodium
 
 def main : IO Unit := do
-  IO.println <| "Thanks for running me"
+  IO.println <| "Thanks for running me!"
+  -- Test running an externally defined function
+  IO.println <| "Running an external addition of 1 + 1:"
   IO.println <| myAdd 1 1
