VCVio.lean
@@ -26,6 +26,7 @@ import VCVio.OracleComp.DistSemantics.Seq
 import VCVio.OracleComp.DistSemantics.Support
 import VCVio.OracleComp.OracleAlg
 import VCVio.OracleComp.OracleComp
+import VCVio.OracleComp.OracleImpl
 import VCVio.OracleComp.OracleSpec
 import VCVio.OracleComp.QueryBound
 import VCVio.OracleComp.RunIO
