VCVio/CryptoFoundations/FiatShamir.lean
@@ -18,40 +18,48 @@ For simplicity we construct signature schemes rather than general proofs of know
 -- TODO
 open OracleComp OracleSpec
 
-variable {ι : Type} (spec : ℕ → OracleSpec ι)
-    (X W : ℕ → Type) (p : {n : ℕ} → X n → W n → Bool)
-    (PC SC Ω P M : ℕ → Type)
-    [Π n, Inhabited (Ω n)] [Π n, DecidableEq (Ω n)]
-    [Π n, Fintype (Ω n)] [Π n, SelectableType (Ω n)]
-    [Π n, DecidableEq (PC n)] [Π n, DecidableEq (M n)]
-    [Π n, Fintype (X n)] [Π n, Inhabited (X n)] [Π n, SelectableType (X n)]
-    [Π n, Fintype (W n)] [Π n, Inhabited (W n)] [Π n, SelectableType (W n)]
+-- variable {ι : Type} (spec : ℕ → OracleSpec ι)
+--     (X W : ℕ → Type) (p : {n : ℕ} → X n → W n → Bool)
+--     (PC SC Ω P M : ℕ → Type)
+--     [Π n, Inhabited (Ω n)] [Π n, DecidableEq (Ω n)]
+--     [Π n, Fintype (Ω n)] [Π n, SelectableType (Ω n)]
+--     [Π n, DecidableEq (PC n)] [Π n, DecidableEq (M n)]
+--     [Π n, Fintype (X n)] [Π n, Inhabited (X n)] [Π n, SelectableType (X n)]
+--     [Π n, Fintype (W n)] [Π n, Inhabited (W n)] [Π n, SelectableType (W n)]
 
-/-- Given a Σ-protocol we get a signature algorithm by using a random oracle to generate
-challenge values for the Σ-protocol, including the message in the hash input. -/
-def FiatShamir (sigmaAlg : SigmaAlg (λ n ↦ spec n) X W p PC SC Ω P)
-    (hr : GenerableRelation spec X W p) :
-    SignatureAlg (λ n ↦ spec n ++ₒ (M n × PC n →ₒ Ω n))
-      (M := M) (PK := X) (SK := W)
-      (S := λ n ↦ PC n × P n) where
-  -- Use the existing algorithm for generating relation members
-  keygen := λ n ↦ hr.gen n
-  -- Sign by running the sigma protocol using a hash as the challenge
-  sign := λ n pk sk m ↦ do
-    let (c, e) ← sigmaAlg.commit n pk sk
-    let r ← query (Sum.inr <| Sum.inr ()) (m, c)
-    let s ← sigmaAlg.respond n pk sk e r
-    return (c, s)
-  -- Verify a signature by checking the challenge returned by the random oracle
-  verify := λ n pk m (c, s) ↦ do
-    let r' ← query (Sum.inr <| Sum.inr ()) (m, c)
-    return sigmaAlg.verify n pk c r' s
-  -- Simulation includes an additional cache for random oracle
-  baseState := λ n ↦ sigmaAlg.baseState n × QueryCache _
-  -- Add an empty cache to initial state
-  init_state := λ n ↦ (sigmaAlg.init_state n, ∅)
-  -- Simulate the additional oracle as a random oracle
-  baseSimOracle := λ n ↦ sigmaAlg.baseSimOracle n ++ₛₒ randOracle
+variable {ι : Type} {spec : OracleSpec ι} {σ X W : Type}
+    {p : X → W → Bool} {PC SC Ω P : Type}
+
+
+-- /-- Given a Σ-protocol we get a signature algorithm by using a random oracle to generate
+-- challenge values for the Σ-protocol, including the message in the hash input. -/
+-- def FiatShamirTransform (sigmaAlg : SigmaAlg spec σ X W p PC SC Ω P)
+--     (M : Type) :
+--     SignatureAlg spec σ M X W (PC × P) := sorry
+
+-- def FiatShamir (sigmaAlg : SigmaAlg (λ n ↦ spec n) X W p PC SC Ω P)
+--     (hr : GenerableRelation spec X W p) :
+--     SignatureAlg (λ n ↦ spec n ++ₒ (M n × PC n →ₒ Ω n))
+--       (M := M) (PK := X) (SK := W)
+--       (S := λ n ↦ PC n × P n) where
+--   -- Use the existing algorithm for generating relation members
+--   keygen := λ n ↦ hr.gen n
+--   -- Sign by running the sigma protocol using a hash as the challenge
+--   sign := λ n pk sk m ↦ do
+--     let (c, e) ← sigmaAlg.commit n pk sk
+--     let r ← query (Sum.inr <| Sum.inr ()) (m, c)
+--     let s ← sigmaAlg.respond n pk sk e r
+--     return (c, s)
+--   -- Verify a signature by checking the challenge returned by the random oracle
+--   verify := λ n pk m (c, s) ↦ do
+--     let r' ← query (Sum.inr <| Sum.inr ()) (m, c)
+--     return sigmaAlg.verify n pk c r' s
+--   -- Simulation includes an additional cache for random oracle
+--   baseState := λ n ↦ sigmaAlg.baseState n × QueryCache _
+--   -- Add an empty cache to initial state
+--   init_state := λ n ↦ (sigmaAlg.init_state n, ∅)
+--   -- Simulate the additional oracle as a random oracle
+--   baseSimOracle := λ n ↦ sigmaAlg.baseSimOracle n ++ₛₒ randOracle
 
 namespace FiatShamir
 
