VCVio/CryptoFoundations/HardnessAssumptions/HardHomogeneousSpace.lean
@@ -14,41 +14,41 @@ We use mathlib's `AddTorsor` type class to represent the bijection property,
 and extend this with finiteness and decidability conditions
 -/
 
-open OracleSpec OracleComp OracleAlg BigOperators ENNReal
+-- open OracleSpec OracleComp OracleAlg BigOperators ENNReal
 
-class HomogeneousSpace (G : semiOutParam (ℕ → Type)) (P : semiOutParam (ℕ → Type)) where
-  AddGroup_G (sp : ℕ) : AddCommGroup (G sp)
-  AddTorsor_GP (sp : ℕ) : AddTorsor (G sp) (P sp)
-  decidableEq_G (sp : ℕ) : DecidableEq (G sp)
-  decidableEq_P (sp : ℕ) : DecidableEq (P sp)
-  fintype_G (sp : ℕ) : Fintype (G sp)
-  fintype_P (sp : ℕ) : Fintype (P sp)
-  inhabited_G (sp : ℕ) : Inhabited (G sp)
-  inhabited_P (sp : ℕ) : Inhabited (P sp)
-  selectableType_G (sp : ℕ) : SelectableType (G sp)
-  selectableType_P (sp : ℕ) : SelectableType (P sp)
+-- class HomogeneousSpace (G : semiOutParam (ℕ → Type)) (P : semiOutParam (ℕ → Type)) where
+--   AddGroup_G (sp : ℕ) : AddCommGroup (G sp)
+--   AddTorsor_GP (sp : ℕ) : AddTorsor (G sp) (P sp)
+--   decidableEq_G (sp : ℕ) : DecidableEq (G sp)
+--   decidableEq_P (sp : ℕ) : DecidableEq (P sp)
+--   fintype_G (sp : ℕ) : Fintype (G sp)
+--   fintype_P (sp : ℕ) : Fintype (P sp)
+--   inhabited_G (sp : ℕ) : Inhabited (G sp)
+--   inhabited_P (sp : ℕ) : Inhabited (P sp)
+--   selectableType_G (sp : ℕ) : SelectableType (G sp)
+--   selectableType_P (sp : ℕ) : SelectableType (P sp)
 
-namespace HomogeneousSpace
+-- namespace HomogeneousSpace
 
-variable (G P : ℕ → Type)
+-- variable (G P : ℕ → Type)
 
-instance [h : HomogeneousSpace G P] (sp : ℕ) : AddCommGroup (G sp) := h.AddGroup_G sp
-instance [h : HomogeneousSpace G P] (sp : ℕ) : AddTorsor (G sp) (P sp) := h.AddTorsor_GP sp
-instance [h : HomogeneousSpace G P] (sp : ℕ) : DecidableEq (G sp) := h.decidableEq_G sp
-instance [h : HomogeneousSpace G P] (sp : ℕ) : DecidableEq (P sp) := h.decidableEq_P sp
-instance [h : HomogeneousSpace G P] (sp : ℕ) : Fintype (G sp) := h.fintype_G sp
-instance [h : HomogeneousSpace G P] (sp : ℕ) : Fintype (P sp) := h.fintype_P sp
-instance [h : HomogeneousSpace G P] (sp : ℕ) : Inhabited (G sp) := h.inhabited_G sp
-instance [h : HomogeneousSpace G P] (sp : ℕ) : Inhabited (P sp) := h.inhabited_P sp
-instance [h : HomogeneousSpace G P] (sp : ℕ) : SelectableType (G sp) := h.selectableType_G sp
-instance [h : HomogeneousSpace G P] (sp : ℕ) : SelectableType (P sp) := h.selectableType_P sp
+-- instance [h : HomogeneousSpace G P] (sp : ℕ) : AddCommGroup (G sp) := h.AddGroup_G sp
+-- instance [h : HomogeneousSpace G P] (sp : ℕ) : AddTorsor (G sp) (P sp) := h.AddTorsor_GP sp
+-- instance [h : HomogeneousSpace G P] (sp : ℕ) : DecidableEq (G sp) := h.decidableEq_G sp
+-- instance [h : HomogeneousSpace G P] (sp : ℕ) : DecidableEq (P sp) := h.decidableEq_P sp
+-- instance [h : HomogeneousSpace G P] (sp : ℕ) : Fintype (G sp) := h.fintype_G sp
+-- instance [h : HomogeneousSpace G P] (sp : ℕ) : Fintype (P sp) := h.fintype_P sp
+-- instance [h : HomogeneousSpace G P] (sp : ℕ) : Inhabited (G sp) := h.inhabited_G sp
+-- instance [h : HomogeneousSpace G P] (sp : ℕ) : Inhabited (P sp) := h.inhabited_P sp
+-- instance [h : HomogeneousSpace G P] (sp : ℕ) : SelectableType (G sp) := h.selectableType_G sp
+-- instance [h : HomogeneousSpace G P] (sp : ℕ) : SelectableType (P sp) := h.selectableType_P sp
 
-class vectorizationHard (G P : ℕ → Type) [HomogeneousSpace G P]
-    extends HardRelation (λ _ ↦ emptySpec) (λ n ↦ P n × P n) (λ n ↦ G n)
-      (λ (x₁, x₂) g ↦ g = x₁ -ᵥ x₂)
+-- class vectorizationHard (G P : ℕ → Type) [HomogeneousSpace G P]
+--     extends HardRelation (λ _ ↦ emptySpec) (λ n ↦ P n × P n) (λ n ↦ G n)
+--       (λ (x₁, x₂) g ↦ g = x₁ -ᵥ x₂)
 
-class parallelizationHard (G P : ℕ → Type) [HomogeneousSpace G P]
-    extends HardRelation (λ _ ↦ emptySpec) (λ n ↦ P n × P n × P n) (λ n ↦ P n)
-      (λ (x₁, x₂, x₃) x₄ ↦ x₁ -ᵥ x₂ = x₃ -ᵥ x₄)
+-- class parallelizationHard (G P : ℕ → Type) [HomogeneousSpace G P]
+--     extends HardRelation (λ _ ↦ emptySpec) (λ n ↦ P n × P n × P n) (λ n ↦ P n)
+--       (λ (x₁, x₂, x₃) x₄ ↦ x₁ -ᵥ x₂ = x₃ -ᵥ x₄)
 
-end HomogeneousSpace
+-- end HomogeneousSpace
