VCVio/OracleComp/DistSemantics/Seq.lean
@@ -230,4 +230,14 @@ lemma probEvent_seq_map_eq_mul (p : γ → Prop) (q1 : α → Prop) (q2 : β →
 
 end seq_map
 
+-- TODO: should have a map lemmas file probably
+lemma probOutput_map_eq_single {oa : OracleComp spec α} {f : α → β} {y : β}
+    (x : α) (h : ∀ x' ∈ oa.support, y = f x' → x = x') (h' : f x = y) :
+    [= y | f <$> oa] = [= x | oa] := by
+  rw [probOutput_map_eq_tsum]
+  refine (tsum_eq_single x (λ x' hx' ↦ ?_)).trans (by rw [h', probOutput_pure_self, mul_one])
+  specialize h x'
+  simp only [mul_eq_zero, probOutput_eq_zero_iff, support_pure, Set.mem_singleton_iff]
+  tauto
+
 end OracleComp
