VCVio/OracleComp/OracleAlg.lean
@@ -18,83 +18,83 @@ The function `OracleAlg.exec` can then be used to properly "execute" a compuatio
 according to the specified simulation oracle
 -/
 
-open OracleSpec OracleComp
+-- open OracleSpec OracleComp
 
-structure OracleAlg {ι : Type} (spec : ℕ → OracleSpec ι) where
-  baseState (n : ℕ) : Type
-  init_state (n : ℕ) : baseState n
-  baseSimOracle (n : ℕ) : spec n →[baseState n]ₛₒ unifSpec
+-- structure OracleAlg {ι : Type} (spec : ℕ → OracleSpec ι) where
+--   baseState (n : ℕ) : Type
+--   init_state (n : ℕ) : baseState n
+--   baseSimOracle (n : ℕ) : spec n →[baseState n]ₛₒ unifSpec
 
-namespace OracleAlg
+-- namespace OracleAlg
 
-variable {ι : Type} {spec : ℕ → OracleSpec ι} {α β γ : Type}
-  (alg : OracleAlg spec) (n : ℕ)
+-- variable {ι : Type} {spec : ℕ → OracleSpec ι} {α β γ : Type}
+--   (alg : OracleAlg spec) (n : ℕ)
 
+-- -- def exec (alg : OracleAlg spec) (n : ℕ)
+-- --     (oa : OracleComp (spec n) α) : ProbComp α :=
+-- --   simulate' (alg.baseSimOracle n) (alg.init_state n) oa
+
+-- -- TODO: Could think about basing things around this instead
 -- def exec (alg : OracleAlg spec) (n : ℕ)
---     (oa : OracleComp (spec n) α) : ProbComp α :=
---   simulate' (alg.baseSimOracle n) (alg.init_state n) oa
+--     (oa : OracleComp (unifSpec ++ₒ spec n) α) : ProbComp α :=
+--   simulate' (idOracle ++ₛₒ alg.baseSimOracle n) ((), alg.init_state n) oa
 
--- TODO: Could think about basing things around this instead
-def exec (alg : OracleAlg spec) (n : ℕ)
-    (oa : OracleComp (unifSpec ++ₒ spec n) α) : ProbComp α :=
-  simulate' (idOracle ++ₛₒ alg.baseSimOracle n) ((), alg.init_state n) oa
+-- -- lemma exec_def (oa : OracleComp (spec n) α) :
+-- --     alg.exec n oa = simulate' (alg.baseSimOracle n) (alg.init_state n) oa := rfl
 
--- lemma exec_def (oa : OracleComp (spec n) α) :
---     alg.exec n oa = simulate' (alg.baseSimOracle n) (alg.init_state n) oa := rfl
+-- lemma exec_def (oa : OracleComp (unifSpec ++ₒ spec n) α) :
+--     alg.exec n oa = simulate' (idOracle ++ₛₒ alg.baseSimOracle n) ((), alg.init_state n) oa :=
+--   rfl
 
-lemma exec_def (oa : OracleComp (unifSpec ++ₒ spec n) α) :
-    alg.exec n oa = simulate' (idOracle ++ₛₒ alg.baseSimOracle n) ((), alg.init_state n) oa :=
-  rfl
+-- -- @[simp low]
+-- -- lemma exec_return (x : α) : alg.exec n (return x) = return x := rfl
 
 -- @[simp low]
--- lemma exec_return (x : α) : alg.exec n (return x) = return x := rfl
+-- lemma exec'_pure (x : α) : alg.exec n (pure x) = pure x := rfl
 
-@[simp low]
-lemma exec'_pure (x : α) : alg.exec n (pure x) = pure x := rfl
+-- -- @[simp low]
+-- -- lemma exec_bind (oa : OracleComp (spec n) α) (ob : α → OracleComp (spec n) β) :
+-- --     alg.exec n (oa >>= ob) = (do
+-- --       let (x, s) ← simulate (alg.baseSimOracle n) (alg.init_state n) oa
+-- --       simulate' (alg.baseSimOracle n) s (ob x)) :=
+-- --   simulate'_bind (alg.baseSimOracle n) (alg.init_state n) oa ob
 
--- @[simp low]
--- lemma exec_bind (oa : OracleComp (spec n) α) (ob : α → OracleComp (spec n) β) :
---     alg.exec n (oa >>= ob) = (do
---       let (x, s) ← simulate (alg.baseSimOracle n) (alg.init_state n) oa
---       simulate' (alg.baseSimOracle n) s (ob x)) :=
---   simulate'_bind (alg.baseSimOracle n) (alg.init_state n) oa ob
+-- -- @[simp low]
+-- -- lemma exec_query (alg : OracleAlg spec) (i : ι) (t : (spec n).domain i) :
+-- --     alg.exec n (query i t) = Prod.fst <$> alg.baseSimOracle n i t (alg.init_state n) :=
+-- --   simulate'_query (alg.baseSimOracle n) (alg.init_state n) i t
 
--- @[simp low]
--- lemma exec_query (alg : OracleAlg spec) (i : ι) (t : (spec n).domain i) :
---     alg.exec n (query i t) = Prod.fst <$> alg.baseSimOracle n i t (alg.init_state n) :=
---   simulate'_query (alg.baseSimOracle n) (alg.init_state n) i t
+-- -- @[simp low]
+-- -- lemma exec_map (alg : OracleAlg spec) (oa : OracleComp (spec n) α) (f : α → β) :
+-- --     alg.exec n (f <$> oa) = f <$> alg.exec n oa :=
+-- --   simulate'_map (alg.baseSimOracle n) (alg.init_state n) oa f
 
--- @[simp low]
--- lemma exec_map (alg : OracleAlg spec) (oa : OracleComp (spec n) α) (f : α → β) :
---     alg.exec n (f <$> oa) = f <$> alg.exec n oa :=
---   simulate'_map (alg.baseSimOracle n) (alg.init_state n) oa f
+-- -- @[simp low]
+-- -- lemma exec_seq (alg : OracleAlg spec) (oa : OracleComp (spec n) α)
+-- --     (og : OracleComp (spec n) (α → β)) : alg.exec n (og <*> oa) = (do
+-- --       let (f, s) ← simulate (alg.baseSimOracle n) (alg.init_state n) og
+-- --       f <$> simulate' (alg.baseSimOracle n) s oa) :=
+-- --   simulate'_seq (alg.baseSimOracle n) (alg.init_state n) oa og
 
--- @[simp low]
--- lemma exec_seq (alg : OracleAlg spec) (oa : OracleComp (spec n) α)
---     (og : OracleComp (spec n) (α → β)) : alg.exec n (og <*> oa) = (do
---       let (f, s) ← simulate (alg.baseSimOracle n) (alg.init_state n) og
---       f <$> simulate' (alg.baseSimOracle n) s oa) :=
---   simulate'_seq (alg.baseSimOracle n) (alg.init_state n) oa og
+-- section baseOracleAlg
 
-section baseOracleAlg
+-- /-- Simple base structure for defining algorithms using only uniform selection oracles.
+-- Usefull to auto-fill in fields with simple defaults in this case. -/
+-- -- abbrev baseOracleAlg : OracleAlg (λ _ ↦ unifSpec) where
+-- --   baseState := λ _ ↦ Unit
+-- --   init_state := λ _ ↦ ()
+-- --   baseSimOracle := λ _ ↦ idOracle
 
-/-- Simple base structure for defining algorithms using only uniform selection oracles.
-Usefull to auto-fill in fields with simple defaults in this case. -/
--- abbrev baseOracleAlg : OracleAlg (λ _ ↦ unifSpec) where
+-- abbrev baseOracleAlg : OracleAlg (λ _ ↦ []ₒ) where
 --   baseState := λ _ ↦ Unit
 --   init_state := λ _ ↦ ()
---   baseSimOracle := λ _ ↦ idOracle
+--   baseSimOracle := λ _ ↦ unifOracle
 
-abbrev baseOracleAlg : OracleAlg (λ _ ↦ []ₒ) where
-  baseState := λ _ ↦ Unit
-  init_state := λ _ ↦ ()
-  baseSimOracle := λ _ ↦ unifOracle
+-- -- @[simp]
+-- -- lemma exec_baseOracleAlg (n : ℕ) (oa : ProbComp α) :
+-- --     baseOracleAlg.exec n oa = oa := by
+-- --   simp only [exec_def, idOracle.simulate'_eq]
 
--- @[simp]
--- lemma exec_baseOracleAlg (n : ℕ) (oa : ProbComp α) :
---     baseOracleAlg.exec n oa = oa := by
---   simp only [exec_def, idOracle.simulate'_eq]
+-- end baseOracleAlg
 
-end baseOracleAlg
-
-end OracleAlg
+-- end OracleAlg
