VCVio/OracleComp/OracleImpl.lean
@@ -1,0 +1,58 @@
+/-
+Copyright (c) 2024 Devon Tuma. All rights reserved.
+Released under Apache 2.0 license as described in the file LICENSE.
+Authors: Devon Tuma
+-/
+import VCVio.OracleComp.SimSemantics.Constructions
+
+/-!
+# Implementations of Oracles
+
+This file defines a structure `OracleImpl spec σ` that represents a specification of
+how to run the oracles in `spec` using only probabalistic computations.
+The type `σ` is the state used in the implementation (e.g. a random oracle's cache).
+
+We implement this a structure so that the types of protocols can extend it,
+allowing the main definition to be oracle agnostic.
+-/
+
+open OracleSpec OracleComp
+
+/-- An implementation of the oracles in `spec` gives a way to run all the oracles in `spec`.
+Allows a computation using `spec` to be simulated in terms of `unifSpec` to produce
+a `ProbComp` that can be run with `OracleComp.runIO`.
+
+The types of primitives can extend this to ensure that any oracles used in a protocol
+must have some canonical implementation. -/
+structure OracleImpl {ι : Type} (spec : OracleSpec ι) (σ : Type) where
+  /-- Simulation oracle giving an implementation of the oracles in `spec`. -/
+  baseSimOracle : spec →[σ]ₛₒ unifSpec
+  init_state : σ
+
+namespace OracleImpl
+
+variable {ι : Type} {spec : OracleSpec ι} {σ α β γ : Type}
+
+/-- Run a computation `oa` using a given implementation `impl` of its oracles,
+with initial state `s`. Returns both the result and final state.
+The computation `oa` is assumed to also have access to uniform selection oracles,
+which are simulated by directly forwarding their calls with `idOracle`. -/
+abbrev run (impl : OracleImpl spec σ) (s : σ)
+    (oa : OracleComp spec α) : ProbComp (α × σ) :=
+  simulate impl.baseSimOracle s oa
+
+abbrev exec (impl : OracleImpl spec σ)
+    (oa : OracleComp spec α) : ProbComp (α × σ) :=
+  simulate impl.baseSimOracle impl.init_state oa
+
+/-- Impliment an empty set of oracles by eliminating on the empty index to any queries. -/
+@[simps] def emptyImpl : OracleImpl []ₒ Unit where
+  baseSimOracle := unifOracle
+  init_state := ()
+
+/-- Implement `unifSpec` as `unifSpec` by identity. -/
+@[simps] def defaultImpl : OracleImpl unifSpec Unit where
+  baseSimOracle := idOracle
+  init_state := ()
+
+end OracleImpl
